Move exp.subst.{update,apply} to own files, remove unused theorems
Remove exp.subst.{update_distrib,apply_distrib}

src/exp/subst/update.lean
@@ -1,6 +1,6 @@
 /-
 
-This files defines core `subst` definitions.
+This files defines the `subst.update` definition and theorems.
 
 -/
 
@@ -12,9 +12,10 @@ namespace exp ------------------------------------------------------------------
 namespace subst ----------------------------------------------------------------
 
 variables {V : Type} [decidable_eq V] -- Type of variable names
-variables {a : V} -- Variable names
+variables {a b : V} -- Variable names
 variables {vs : Type → Type} [vset vs V] -- Type of variable name sets
 variables {X Y : vs V} -- Variable name sets
+variables {F : subst X Y} -- Substitutions
 
 -- Update a given substitution with a new variable substitution
 @[reducible]
@@ -26,29 +27,41 @@ def update (a b : V) (F : subst X Y) : subst (insert a X) (insert b Y) :=
   else
     insert_var b (F (vname.erase x p))
 
+namespace update ---------------------------------------------------------------
+
 protected
-theorem update.eq {a b : V} {F : subst X Y} (x : ν∈ insert a X) (p : x.1 = a)
+theorem eq (x : ν∈ insert a X) (p : x.1 = a)
 : subst.update a b F x = var (vname.insert_self b Y) :=
   by simp [subst.update, dif_pos p]
 
 protected
-theorem update.eq_self {a b : V} {F : subst X Y}
+theorem eq_self
 : subst.update a b F (vname.insert_self a X) = var (vname.insert_self b Y) :=
   update.eq (vname.insert_self a X) rfl
 
 protected
-theorem update.ne {a b : V} (F : subst X Y) (x : ν∈ insert a X) (p : x.1 ≠ a)
+theorem ne (F : subst X Y) (x : ν∈ insert a X) (p : x.1 ≠ a)
 : subst.update a b F x = insert_var b (F (vname.erase x p)) :=
   by simp [subst.update, dif_neg p]
 
--- Apply a substitution to one expression to get another with different free
--- variables.
-@[reducible]
 protected
-def apply : ∀ {X Y : vs V}, subst X Y → exp X → exp Y
-  | X Y F (var x)    := F x
-  | X Y F (app f e)  := app (apply F f) (apply F e)
-  | X Y F (lam' a e) := lam (apply (subst.update a (fresh Y).1 F) e)
+theorem lift (a b : V) (F : X →ν Y)
+: subst.update a b (subst.lift F) = subst.lift (vname.update a b F) :=
+  begin
+    funext x,
+    cases x with c pc,
+    simp [subst.update, subst.lift, function.comp, vname.update],
+    cases decidable.em (c = a) with c_eq_a c_ne_a,
+    begin /- c_eq_a : c = a -/
+      simp [dif_pos c_eq_a]
+    end,
+    begin /- c_ne_a : c ≠ a -/
+      simp [dif_neg c_ne_a, insert_var, map, vname.insert],
+      reflexivity
+    end
+  end
+
+end /- namespace -/ update -----------------------------------------------------
 
 end /- namespace -/ subst ------------------------------------------------------
 end /- namespace -/ exp --------------------------------------------------------
