src/exp/subst/apply.lean
@@ -1,0 +1,27 @@
+/-
+
+This files defines `subst.apply`.
+
+-/
+
+import .update
+
+namespace acie -----------------------------------------------------------------
+namespace exp ------------------------------------------------------------------
+namespace subst ----------------------------------------------------------------
+
+variables {V : Type} [decidable_eq V] -- Type of variable names
+variables {vs : Type → Type} [vset vs V] -- Type of variable name sets
+
+-- Apply a substitution to one expression to get another with different free
+-- variables.
+@[reducible]
+protected
+def apply : ∀ {X Y : vs V}, subst X Y → exp X → exp Y
+  | X Y F (var x)    := F x
+  | X Y F (app f e)  := app (apply F f) (apply F e)
+  | X Y F (lam' a e) := lam (apply (subst.update a (fresh Y).1 F) e)
+
+end /- namespace -/ subst ------------------------------------------------------
+end /- namespace -/ exp --------------------------------------------------------
+end /- namespace -/ acie -------------------------------------------------------
